---
title: "math"
date: 2022-03-15T23:43:58+08:00
draft: false
math: true
---

$$f(a)=\frac{1}{\tau i}\oint_\gamma\frac{f(z)}{z-a}\mathrm{d}z$$

$$\left(x+\frac{D}{2}\right)^2+\left(y+\frac{E}{2}\right)^2=\left(\frac{D}{2}\right)^2+\left(\frac{E}{2}\right)^2-F$$

$$S=\frac{x\sin\left(\frac{\tau}{x}\right)k^2}{4(1-\cos\left(\frac{\tau}{x}\right))}$$

$$\frac{2 \sqrt{A_0^2+B_0^2} \sqrt{A_0^2 (E^2-C F)+B_0^2 (D^2-A F)+C_0^2 (B^2-A C)+2( A_0 B_0 B F+ A_0 C_0 C D+ B_0 C_0 A E- A_0 B_0 D E- A_0 C_0 B E- B_0 C_0 B D)}}{A_0^2 C+B_0^2 A -2 A_0 B_0 B}$$

$$\frac{2 \sqrt{A_0^2+B_0^2} \sqrt{A_0^2 (E^2)+B_0^2 (D^2)-C_0^2 A C)+2(A_0 C_0 C D+ B_0 C_0 A E- A_0 B_0 D E)}}{A_0^2 C+B_0^2 A}$$

$$Cy^2+2Dx=0$$

$$\frac{2 \sqrt{A_0^2+B_0^2} \sqrt{B_0^2 D^2+2A_0 C_0 C D}}{A_0^2 C}$$

$$Ax^2+2Ex=0$$

$$\frac{2 \sqrt{A_0^2+B_0^2} \sqrt{A_0^2 E^2+2B_0 C_0 A E}}{B_0^2 A}$$

$$A=\frac{\tau}{2}\frac{\frac{D^2}{A}+\frac{E^2}{C}-F}{\sqrt{AC}}$$

$$(Ax_0+By_0+D)(x-x_0)+(Cy_0+Bx_0+E)(y-y_0)=0$$

$$\left(\frac{CD-BE}{B^2-AC},\frac{AE-BD}{B^2-AC}\right)$$

$$e^2=\frac{2\sqrt{(A-C)^2+4B^2}}{\eta(A+C)+\sqrt{(A-C)^2+B^2}},\eta=\left\\{\begin{matrix}
1 & e < 1\\\\
-1 & e \geq 1
\end{matrix}\right.$$

$$x_1+x_2 =\frac{2(B_0 C_0 B + A_0 B_0 E - A_0 C_0 C - B_0^2 D)}{A_0^2 C + B_0^2 A -2 A_0 B_0 B}$$

$$y_1 + y_2 = \frac{2(A_0 C_0 B + A_0 B_0 D - B_0 C_0 A - A_0^2 E)}{A_0^2 C + B_0^2 A -2 A_0 B_0 B}$$

$$x_1 x_2 = \frac{C_0^2 C + B_0^2 F - 2 B_0 C_0 E}{A_0^2 C + B_0^2 A - 2 A_0 B_0 B}$$

$$y_1 y_2 = \frac{C_0^2 A + 2 A_0^2 F - 2 A_0 C_0 D}{A_0^2 C + B_0^2 A - 2 A_0 B_0 B}$$

$$Axx_0+B(x_0y+xy_0)+Cyy_0+D(x+x_0)+E(y-y_0)+F=0$$

$$(X,Y)=\left(\frac{x}{1-z},\frac{y}{1-z}\right)$$
$$(x,y,z)=\left(\frac{2X}{X^2+Y^2+1},\frac{2Y}{X^2+Y^2+1},\frac{X^2+Y^2-1}{X^2+Y^2+1}\right)$$
