---
title: "Math in NCEE"
date: 2022-07-12T00:17:50+08:00
draft: false
math: true
---

## Quadratic functions

$$\left(x+\frac{b}{2a}\right)^2=\left(\frac{b}{2a}\right)^2-\frac{c}{a}$$

$$f(x)=a(x-h)^2+k=a(x-x_1)(x-x_2)$$

$$f(x)=a(x-x_0)^2+(kx+d)$$

$$x=-\frac{b}{2a}=\frac{x_1+x_2}{2}$$

$$\left(-\frac{b}{2a},c-\frac{b^2}{4a}\right)$$

## Functions

|$$f(x)$$|$$T$$|
|--|--|
|$$f(x+T)=f(x)$$|$$T$$|
|$$f(x+T)=-f(x)$$|$$2T$$|
|$$f(x+m)=f(x+n)$$|$$2\|m-n\|$$|
|$$f(x+T)=-\frac{1}{f(x)}$$|$$2T$$|


### axial symmetry
|$$f(x)$$|axial|
|--|--|
|$$f(x+a)=f(b-x)$$|$$\frac{a+b}{2}$$|
|$$y=f(x+a),y=f(b-x)$$|$$\frac{b-a}{2}$$|


$$\sqrt{a}\sqrt{b}=\sqrt{ab}$$
$$\sqrt{\frac{a}{b}}=\frac{\sqrt{a}}{\sqrt{b}}=\frac{\sqrt{ab}}{b}$$
$$a^{\frac{m}{n}}=\sqrt[n]{a^m}$$
$$a^{-\frac{m}{n}}=\frac{1}{\sqrt[n]{a^m}}$$
$$\log_{a^m}^{b^n}=\frac{n}{m}\log_a b$$

## Absolute

$$a>0,|x|<a \Leftrightarrow -a<x<a$$
$$a>0,|x|>a \Leftrightarrow x<-a\ \mathrm{or}\ x>a$$
$$c>0,|ax+b|<c \Leftrightarrow -c < ax+b < c$$
$$c>0,|ax+b|>c \Leftrightarrow ax+b >c\ \mathrm{or}\ ax+b < -c$$


## Trigonometric functions

$$1 \approx 57^\circ$$
$$c=2\pi r$$
$$S=\pi r^2$$
$$l=|a|r$$
$$S=\frac{1}{2}lr=\frac{1}{2}|a|r^2$$

## Calculus

|$$f(x)$$|$$f(x)'$$|
|--|--|
|$$c$$|$$0$$|
|$$x^a$$|$$ax^{a-1}$$|
|$$\sin x$$|$$\cos x$$|
|$$\cos x$$|$$-\sin x$$|
|$$a^x$$|$$a^x \ln a$$|
|$$e^x$$|$$e^x$$|
|$$\log_a x$$|$$\frac{1}{x\ln a}$$|
|$$\ln x$$|$$\frac{1}{x}$$|

$$(uv)'=u'v+uv'$$

$$\left(\frac{u}{v}\right)=\frac{u'v-uv'}{v^2}$$

## Inequalities

$$a+b\geq 2\sqrt{ab}$$

$$a^2+b^2\geq 2ab$$

$$ab\leq\left(\frac{a+b}{2}\right)^2\leq\frac{a^2+b^2}{2}$$

## Trigonometry

## Conic section

## Geometry

## Series

|Arithmetico sequence|Geometric sequence|
|--|--|
|$$a_n=a_0+nd=a_m+(n-m)d$$|$$a_n=a_0 q^n=a_mq^{n-m}$$|
|$$S_n=na_0+\frac{n(n+1)}{2}d=\frac{n(a_1+a_n)}{2}$$|$$S_n=a_0q\frac{q^n-1}{q-1}=\frac{a_nq-a_1}{q-1}$$|
|$$T_n=\frac{d^n\left(n+\frac{a_0}{d}\right)!}{\left(\frac{a_0}{d}\right)!}$$|$$T_n=a_0^n q^{\frac{n(n+1)}{2}}$$|
|$$S_{(n+1)k}-S_{nk}=k(a_0+\frac{k+1}{2}d)+dk^2n$$|$$S_{(n+1)k}-S_{nk}=a_0\frac{q^k-1}{q-1}q^{kn+1}$$|

$$S_n=\frac{A_1G_1-A_{n+1}G_{n+1}}{1-r}+\frac{dr}{(1-r)^2}\left(G_1-G_{n+1}\right)$$

$$\sum_{x=1}^n A_{1_n} A_{2_n} = d_1d_2\frac{n^3}{2}+\left(a_0d_2+b_0d_1+d_1d_2\right)\frac{n^2}{2}+\left(6a_0b_0+3a_0d_2+3b_0d_1+d_1d_2\right)\frac{n}{6}$$

$$\sum_{x=1}^n G_{1_n} G_{2_n} = \frac{a_0b_0q_1q_2(q_1^nq_2^n-1)}{q_1q_2-1}$$

$$\frac{S_n}{n}=a_0+\frac{n+1}{2}d$$

$$\frac{1}{a_n}=\frac{1}{a_1+(n-1)d}$$
$$S_n=\frac{1}{d}\ln\left(1+n\frac{2d}{2a_0+d}\right)$$

$$\sum_{k=1}^n\left[a_1+(k-1)d\right]r^{k-1}=\frac{a-[a+(n-1)d]r^n}{1-r}+\frac{dr(1-r^{n-1})}{(1-r)^2}$$

$$\frac{1}{n(n-k)}=\frac{1}{k}\left(\frac{1}{n}-\frac{1}{n+k}\right)$$
$$\frac{1}{4n^2-1}=\frac{1}{2}\left(\frac{1}{2n-1}-\frac{1}{2n+1}\right)$$
$$\frac{1}{\sqrt{n}+\sqrt{n+m}}=\frac{\sqrt{n+m}-\sqrt{n}}{m}$$
$$\log_a\left(1+\frac{1}{n}\right)=\log_a(n-1)-\log_a n$$


## Vector

## Combinatorics
